SP1Chips/SubChip.lean
@@ -13,64 +13,22 @@ namespace Sub
 variable
   (Main : Vector (Fin KB) 34)
   (s : SailState)
-  -- (cstrs : (constraints Main).allHold)
-  -- (h_is_real : Main[32] = 1)
 
 noncomputable def spec_sub (rs2 rs1 rd : regidx) : SailM Unit := do
   Sail.writeReg Register.nextPC ((← Sail.readReg Register.PC) + 4#64)
   _ ← execute_RTYPE rs2 rs1 rd rop.SUB
   pure ()
 
-def sp1_op_a : BitVec 5 :=
-  by
-    refine BitVec.ofNat 5 Main[6]
-    -- simp
-    -- show Main[6] < 32
+def sp1_op_a : BitVec 5 := BitVec.ofNat 5 Main[6]
 
-    -- have reader_cstrs := by
-    --   simp [SP1ConstraintList.allHold, constraints, SP1Constraint.toProp] at cstrs
-    --   exact cstrs.2.2.1
+def sp1_op_b : BitVec 5 := BitVec.ofNat 5 Main[14]
 
-    -- clear cstrs
-    -- simp [RTypeReader.constraints, h_is_real, Opcode.ofNat, Nat.ble, Nat.beq,
-    --   SP1Constraint.toProp, sub_eq_zero] at reader_cstrs
-    -- simp_all
-    -- exact reader_cstrs.1.2.1
-
-def sp1_op_b : BitVec 5 :=
-  by
-    refine BitVec.ofNat 5 Main[14]
-    -- simp
-    -- show Main[14] < 32
-
-    -- have reader_cstrs := by
-    --   simp [SP1ConstraintList.allHold, constraints, SP1Constraint.toProp] at cstrs
-    --   exact cstrs.2.2.1
-
-    -- clear cstrs
-    -- simp [RTypeReader.constraints, h_is_real, Opcode.ofNat, Nat.ble, Nat.beq, SP1Constraint.toProp] at reader_cstrs
-
-    -- exact reader_cstrs.1.1.1
-
-def sp1_op_c : BitVec 5 :=
-  by
-    refine BitVec.ofNat 5 Main[21]
-    -- simp
-    -- show Main[21] < 32
-
-    -- have reader_cstrs := by
-    --   simp [SP1ConstraintList.allHold, constraints, SP1Constraint.toProp] at cstrs
-    --   exact cstrs.2.2.1
-
-    -- clear cstrs
-    -- simp [RTypeReader.constraints, h_is_real, Opcode.ofNat, Nat.ble, Nat.beq, SP1Constraint.toProp] at reader_cstrs
-
-    -- exact reader_cstrs.1.1.2
+def sp1_op_c : BitVec 5 := BitVec.ofNat 5 Main[21]
 
 def sp1_sub : SailM Unit := do
   let op_a := sp1_op_a Main --cstrs h_is_real
   Sail.writeReg Register.nextPC (Word.toBitVec64 #v[Main[3] + 4, Main[4], Main[5], 0])
-  Sail.write_reg op_a (Word.toBitVec64 #v[Main[28], Main[29], Main[30], Main[31]])
+  Sail.write_reg op_a (Word.toBitVec64 #v[Main[29], Main[30], Main[31], Main[32]])
 
 open Sail
 
@@ -78,9 +36,9 @@ theorem correct_sub
   (cstrs : (constraints Main).allHold)
   (h_is_real : Main[33] = 1)
   (state_cstrs : (constraints Main).initialState s) :
-  let op_c := sp1_op_c Main --cstrs h_is_real
-  let op_b := sp1_op_b Main --cstrs h_is_real
-  let op_a := sp1_op_a Main --cstrs h_is_real
+  let op_c := sp1_op_c Main
+  let op_b := sp1_op_b Main
+  let op_a := sp1_op_a Main
   (spec_sub (.Regidx op_c) (.Regidx op_b) (.Regidx op_a)).run s = (sp1_sub Main ).run s
   := by
     simp [SP1ConstraintList.initialState, constraints, SP1Constraint.toStateProp, List.Forall, SubOperation.constraints, CPUState.constraints, RTypeReader.constraints, h_is_real] at state_cstrs
@@ -91,14 +49,13 @@ theorem correct_sub
     simp [RTypeReader.allHold_constraints_iff_is_real h_is_real,
       Opcode.ofNat, Nat.ble, Nat.beq] at reader_cstrs
 
-    stop
-    obtain ⟨ trusted_instr_prop, _, _, _, _, _, _, ⟨ ⟨ _, _, ⟨ _, is_U64_b, is_U64_c ⟩ ⟩, _ ⟩⟩ := reader_cstrs
+    obtain ⟨ _, trusted_instr_prop, _, _, _, _, _, _, ⟨ ⟨ _, _, ⟨ _, is_U64_b, is_U64_c ⟩ ⟩, _ ⟩⟩ := reader_cstrs
     simp [Opcode.ofNat, Nat.ble, Nat.beq] at trusted_instr_state trusted_instr_prop
 
     rw [h_is_real] at *
     apply SubOperation.spec is_U64_b is_U64_c at sub_op_cstrs
     obtain ⟨ is_U64_val, is_sub ⟩ := sub_op_cstrs
-    simp at *
+    simp [BitVec.ofNatLT_eq_ofNat] at *
 
     -- Now the monadic manipulation
     simp [spec_sub, sp1_sub, execute, execute_RTYPE']
@@ -111,8 +68,8 @@ theorem correct_sub
     by_cases h_is_op_a_0 : Main[6] = 0 <;> simp_all
     . rw [← is_sub]
       simp [Word.toBitVec64, Word.toNat]
-    . rw [if_neg (by simpa [← BitVec.toNat_inj])]
-      rw [if_neg (by simpa [← BitVec.toNat_inj])]
+    . rw [if_neg (by simp [← BitVec.toNat_inj]; omega)]
+      rw [if_neg (by simp [← BitVec.toNat_inj]; omega)]
       simp [Word.toBitVec64, Word.toNat]
       rfl
 
