SP1Chips/AddiChip.lean
@@ -19,40 +19,13 @@ noncomputable def spec_addi (imm : BitVec 12) (rs1 rd : regidx) : SailM Unit := 
   pure ()
 
 def sp1_op_a : BitVec 5 := BitVec.ofNat 5 Main[6]
-  -- by
-  --   refine BitVec.ofNatLT Main[6] ?_
-  --   simp
-  --   show Main[6] < 32
-
-  --   have reader_cstrs := by
-  --     simp [SP1ConstraintList.allHold, constraints, SP1Constraint.toProp] at cstrs
-  --     exact cstrs.2.2.1
-
-  --   clear cstrs
-  --   simp [ITypeReader.constraints, h_is_real, Opcode.ofNat, Nat.ble, Nat.beq, SP1Constraint.toProp] at reader_cstrs
-  --   simp_all
-
-  --   exact reader_cstrs.1.2.1
 
 def sp1_op_b : BitVec 5 := BitVec.ofNat 5 Main[14]
-  -- by
-  --   refine BitVec.ofNatLT Main[14] ?_
-  --   simp
-  --   show Main[14] < 32
-
-  --   have reader_cstrs := by
-  --     simp [SP1ConstraintList.allHold, constraints, SP1Constraint.toProp] at cstrs
-  --     exact cstrs.2.2.1
-
-  --   clear cstrs
-  --   simp [ITypeReader.constraints, h_is_real, Opcode.ofNat, Nat.ble, Nat.beq, SP1Constraint.toProp] at reader_cstrs
-
-  --   exact reader_cstrs.1.1.1
 
 def sp1_op_c : BitVec 12 := BitVec.ofNat 12 Main[21]
 
 def sp1_addi : SailM Unit := do
-  let op_a := sp1_op_a Main ---cstrs h_is_real
+  let op_a := sp1_op_a Main
   Sail.writeReg Register.nextPC (Word.toBitVec64 #v[Main[3] + 4, Main[4], Main[5], 0])
   Sail.write_reg op_a (Word.toBitVec64 #v[Main[26], Main[27], Main[28], Main[29]])
 
@@ -63,8 +36,8 @@ theorem correct_addi
   (h_is_real : Main[30] = 1)
   (state_cstrs : (constraints Main).initialState s) :
   let op_c := sp1_op_c Main
-  let op_b := sp1_op_b Main --cstrs h_is_real
-  let op_a := sp1_op_a Main --cstrs h_is_real
+  let op_b := sp1_op_b Main
+  let op_a := sp1_op_a Main
   (spec_addi op_c (.Regidx op_b) (.Regidx op_a)).run s = (sp1_addi Main).run s
   := by
     -- Obtain and simplify state and pure constraints
@@ -78,35 +51,8 @@ theorem correct_addi
     specialize read_op_b sorry
     specialize read_op_c sorry
 
-    obtain ⟨ trusted_instr_prop, hcm1, hcm2, c0, c1, c2, c3, h11, h12, h13, h14, h15, h16, h17, h18, h19, h20, ⟨ is_U64_a, is_U64_b, hu64 ⟩⟩ := reader_cstrs
+    obtain ⟨ _, trusted_instr_prop, hcm1, hcm2, c0, c1, c2, c3, h11, h12, h13, h14, h15, h16, h17, h18, h19, h20, ⟨ is_U64_a, is_U64_b, hu64 ⟩⟩ := reader_cstrs
 
-    simp [Opcode.ofNat, Nat.ble] at trusted_instr_prop
-    simp only [BitVec.ofNatLT_eq_ofNat] at *
-    simp [spec_addi, sp1_addi, execute, execute_ITYPE]
-    have hs : s.isInitialized := sorry
-    simp [run_readReg_of_isInitialized _ _ hs]
-    simp [sp1_op_b, read_op_b]
-    simp [sp1_op_c, read_op_c]
-    simp [sp1_op_a]
-    stop
-    by_cases h_is_op_a_0 : Main[6] = 0
-    · simp [h_is_op_a_0]
-      have : #v[Main[26], Main[27], Main[28], Main[29]] = 0 := by sorry
-      simp [this]
-      simp [Word.toBitVec64, Word.toNat]
-      refine congr_arg _ ?_
-
-      rw [Std.ExtDHashMap.get?_eq_some_get] at read_pc
-      simp at read_pc
-      rw [Std.ExtDHashMap.get?_eq_some_get] at read_pc
-      rw [read_pc]
-      erw [Option.some_inj] at read_pc
-      rw [KoalaBear.add4_into_pc_ofNat (by omega)]
-      sorry
-    ·
-      sorry
-
-    stop
     simp_all [Opcode.ofNat, Nat.ble]
     have is_U64_c : Word.isU64 #v[Main[21], Main[22], Main[23], Main[24]]
       := by apply Word.isU64_of_cases c0 c1 c2 c3
@@ -124,18 +70,12 @@ theorem correct_addi
     simp [sp1_op_a]
     rw [KoalaBear.add4_into_pc_ofNat (by omega)]
 
-    by_cases h_is_op_a_0 : Main[6] = 0
-    .
-      -- have h13 : Main[13] = 1 := by sorry
-      -- simp [h13, h_is_op_a_0, Opcode.ofNat, Nat.ble] at *
-      have : #v[Main[26], Main[27], Main[28], Main[29]] = 0 := by sorry
-      simp [h_is_op_a_0, this, Word.toBitVec64, Word.toNat]
-
-    . rw [if_neg (by sorry)]
-      rw [if_neg (by sorry)]
+    by_cases h_is_op_a_0 : Main[6] = 0 <;> simp_all
+    . rw [← is_add] at *
       simp [Word.toBitVec64, Word.toNat]
-      congr 2
-
+    . rw [if_neg (by simp [← BitVec.toNat_inj]; omega)]
+      rw [if_neg (by simp [← BitVec.toNat_inj]; omega)]
+      simp [Word.toBitVec64, Word.toNat]
       rfl
 
 end Addi
