SP1Chips/AddwChip.lean
@@ -52,7 +52,7 @@ theorem correct_addw
     obtain ⟨addw_op_cstrs, cpu_cstrs, alu_cstrs, _⟩ := cstrs
     rw [CPUState.allHold_constraints_iff_is_real h_is_real] at cpu_cstrs
     rw [ALUTypeReader.allHold_constraints_iff_is_real h_is_real] at alu_cstrs
-    obtain ⟨ trusted_instr_prop, _, _, _, _, _, _, _, _, _, _, _, _, _, _, is_U64_a, is_U64_b, is_U64_c , _, _ ⟩ := alu_cstrs
+    obtain ⟨ _, trusted_instr_prop, _, _, _, _, _, _, _, _, _, _, _, _, _, _, is_U64_a, is_U64_b, is_U64_c , _, _ ⟩ := alu_cstrs
     simp [Opcode.ofNat, Nat.ble] at *
     simp_all
 
@@ -134,7 +134,7 @@ theorem correct_addw
     obtain ⟨addw_op_cstrs, cpu_cstrs, alu_cstrs, _ ⟩ := cstrs
     rw [CPUState.allHold_constraints_iff_is_real h_is_real] at cpu_cstrs
     rw [ALUTypeReader.allHold_constraints_iff_is_real h_is_real] at alu_cstrs
-    obtain ⟨ trusted_instr_prop, _, _, ⟨ c0, c1, c2, c3 ⟩, _, _, _, _, _, _, _, _, _, _, _, is_U64_a, is_U64_b, _, _, _ ⟩ := alu_cstrs
+    obtain ⟨ _, trusted_instr_prop, _, _, ⟨ c0, c1, c2, c3 ⟩, _, _, _, _, _, _, _, _, _, _, _, is_U64_a, is_U64_b, _, _, _ ⟩ := alu_cstrs
     simp [Opcode.ofNat, Nat.ble] at *
     simp_all
     have is_U64_c : Word.isU64 #v[Main[21], Main[22], Main[23], Main[24]]
