SP1Foundations/Config.lean
@@ -1,5 +1,8 @@
 import SP1Foundations.Field
 
-/-- dt: should eventually have some struct or something. -/
-@[simp]
-def mprotect_enabled : Unit → Fin KB := fun _ => 0
+/-- dt: this is a hack to semi-resemble eventual goals for the code.
+should be a more general initial config setup for the lemmas with register initialization etc. -/
+
+opaque public_value : Unit → ℕ → Fin KB := fun _ => 0
+
+@[simp] axiom mprotect_disabled : public_value () 151 = 0
