SP1Operations/Reader/ALUTypeReader.lean
@@ -10,6 +10,7 @@ set_option maxHeartbeats 2000000 in
 lemma allHold_constraints_iff :
   List.Forall SP1Constraint.toProp (constraints clk_high clk_low pc opcode instr_field_consts op_a_write_value cols is_real) ↔
     (is_real = 0 ∨ is_real = 1) ∧
+    (cols.is_trusted = is_real) ∧
     (is_real = 0 → cols.imm_c = 0) ∧
     (¬is_real = 0 →
       Opcode.trusted_instr (Opcode.ofNat opcode.val) cols.op_a cols.op_b 0 0 0 cols.op_c[0] cols.op_c[1] cols.op_c[2] cols.op_c[3] 0 cols.imm_c ∧
@@ -23,13 +24,13 @@ lemma allHold_constraints_iff :
       pc[0] < 65536 ∧ pc[1] < 65536 ∧ pc[2] < 65536 ∧
       cols.op_a_memory.access_timestamp.diff_low_limb < 65536 ∧
       cols.op_b_memory.access_timestamp.diff_low_limb < 65536 ∧
-      (clk_low + 2 - cols.op_b_memory.access_timestamp.prev_low - 1 - cols.op_b_memory.access_timestamp.diff_low_limb) * 2130673921 < 256 ∧
-      (clk_low + 3 - cols.op_a_memory.access_timestamp.prev_low - 1 - cols.op_a_memory.access_timestamp.diff_low_limb) * 2130673921 < 256 ∧
+      (clk_low + 3 - cols.op_b_memory.access_timestamp.prev_low - 1 - cols.op_b_memory.access_timestamp.diff_low_limb) * 2130673921 < 256 ∧
+      (clk_low + 4 - cols.op_a_memory.access_timestamp.prev_low - 1 - cols.op_a_memory.access_timestamp.diff_low_limb) * 2130673921 < 256 ∧
       Word.isU64 #v[cols.op_a_memory.prev_value[0], cols.op_a_memory.prev_value[1], cols.op_a_memory.prev_value[2], cols.op_a_memory.prev_value[3]] ∧
       Word.isU64 #v[cols.op_b_memory.prev_value[0], cols.op_b_memory.prev_value[1], cols.op_b_memory.prev_value[2], cols.op_b_memory.prev_value[3]]) ∧
     (is_real - cols.imm_c = 0 ∨ is_real - cols.imm_c - 1 = 0) ∧
     (¬is_real - cols.imm_c = 0 →
-      (clk_low + 1 - cols.op_c_memory.access_timestamp.prev_low - 1 - cols.op_c_memory.access_timestamp.diff_low_limb) * 2130673921 < 256 ∧
+      (clk_low + 2 - cols.op_c_memory.access_timestamp.prev_low - 1 - cols.op_c_memory.access_timestamp.diff_low_limb) * 2130673921 < 256 ∧
       cols.op_c_memory.access_timestamp.diff_low_limb < 65536 ∧
       Word.isU64 #v[cols.op_c_memory.prev_value[0], cols.op_c_memory.prev_value[1], cols.op_c_memory.prev_value[2], cols.op_c_memory.prev_value[3]]) ∧
     (cols.op_a_0 ≠ 0 →
@@ -43,14 +44,33 @@ lemma allHold_constraints_iff :
       cols.op_c_memory.prev_value[2] = cols.op_c[2] ∧
       cols.op_c_memory.prev_value[3] = cols.op_c[3])
    := by
-    stop
-    simp [constraints, sub_eq_zero, SP1Constraint.toProp, Fin.lt_iff_val_lt_val, -Opcode.trusted_instr]
-    intro h_is_real; rcases h_is_real <;> by_cases cols.op_a_0 = 0 <;>
-    by_cases cols.imm_c = 0 <;> simp_all [-Opcode.trusted_instr, and_assoc] <;> aesop
+  simp [constraints, sub_eq_zero, SP1Constraint.toProp, Fin.lt_iff_val_lt_val]
+  intros h_is_real
+  rcases h_is_real with h | h
+  · simp [h]
+    by_cases htrust : cols.is_trusted = 0
+    · simp [htrust]
+      by_cases ha0 : cols.op_a_0 = 0 <;> simp [ha0]
+      · intro himm_c
+        simp [himm_c]
+      · intro himm_c
+        simp [himm_c]
+    · simp [htrust]
+  · simp [h]
+    by_cases htrust : cols.is_trusted = 0
+    · simp [htrust]
+    · simp [htrust, ← @eq_comm _ cols.is_trusted, and_assoc]
+      intros
+      by_cases hop_a_0 : cols.op_a_0 = 0
+      · simp [hop_a_0]
+        aesop
+      · simp [hop_a_0]
+        aesop
 
 set_option maxHeartbeats 1000000 in
 lemma allHold_constraints_iff_is_real (h : is_real = 1) :
   List.Forall SP1Constraint.toProp (constraints clk_high clk_low pc opcode instr_field_consts op_a_write_value cols is_real) ↔
+    (cols.is_trusted = is_real) ∧
     Opcode.trusted_instr (Opcode.ofNat opcode.val) cols.op_a cols.op_b 0 0 0 cols.op_c[0] cols.op_c[1] cols.op_c[2] cols.op_c[3] 0 cols.imm_c ∧
     cols.op_a < 32 ∧
     cols.op_b < 65536 ∧
@@ -62,12 +82,12 @@ lemma allHold_constraints_iff_is_real (h : is_real = 1) :
     pc[0] < 65536 ∧ pc[1] < 65536 ∧ pc[2] < 65536 ∧
     cols.op_a_memory.access_timestamp.diff_low_limb < 65536 ∧
     cols.op_b_memory.access_timestamp.diff_low_limb < 65536 ∧
-    (clk_low + 2 - cols.op_b_memory.access_timestamp.prev_low - 1 - cols.op_b_memory.access_timestamp.diff_low_limb) * 2130673921 < 256 ∧
-    (clk_low + 3 - cols.op_a_memory.access_timestamp.prev_low - 1 - cols.op_a_memory.access_timestamp.diff_low_limb) * 2130673921 < 256 ∧
+    (clk_low + 3 - cols.op_b_memory.access_timestamp.prev_low - 1 - cols.op_b_memory.access_timestamp.diff_low_limb) * 2130673921 < 256 ∧
+    (clk_low + 4 - cols.op_a_memory.access_timestamp.prev_low - 1 - cols.op_a_memory.access_timestamp.diff_low_limb) * 2130673921 < 256 ∧
     Word.isU64 #v[cols.op_a_memory.prev_value[0], cols.op_a_memory.prev_value[1], cols.op_a_memory.prev_value[2], cols.op_a_memory.prev_value[3]] ∧
     Word.isU64 #v[cols.op_b_memory.prev_value[0], cols.op_b_memory.prev_value[1], cols.op_b_memory.prev_value[2], cols.op_b_memory.prev_value[3]] ∧
     (cols.imm_c = 0 →
-      (clk_low + 1 - cols.op_c_memory.access_timestamp.prev_low - 1 - cols.op_c_memory.access_timestamp.diff_low_limb) * 2130673921 < 256 ∧
+      (clk_low + 2 - cols.op_c_memory.access_timestamp.prev_low - 1 - cols.op_c_memory.access_timestamp.diff_low_limb) * 2130673921 < 256 ∧
       cols.op_c_memory.access_timestamp.diff_low_limb < 65536 ∧
       Word.isU64 #v[cols.op_c_memory.prev_value[0], cols.op_c_memory.prev_value[1], cols.op_c_memory.prev_value[2], cols.op_c_memory.prev_value[3]]) ∧
     (¬cols.op_a_0 = 0 →
